refactor

resources.v
@@ -8,93 +8,7 @@ Require Import Resources.type.
 Require Import Resources.value.
 Require Import Resources.memory.
 Require Import Resources.instr.
-
-(** Local State Rules *)
-Inductive step_local : ∀
-(M : Memory) (S : LocalStack) (i : Instr)
-(M' : Memory) (S' : LocalStack), Prop :=
-  | step_mvloc : ∀ {x : LocalVariable} {v : RuntimeValue}
-    {M : Memory} {S : LocalStack},
-    maps_var_to M x v →
-    step_local M S (MvLoc x) (mem_remove M x) (v :: S)
-  | step_cploc : ∀ {x : LocalVariable} {u : UnrestrictedValue}
-    {M : Memory} {S : LocalStack},
-    maps_var_to M x u →
-    step_local M S (CpLoc x) M (val u :: S)
-  | step_stloc_u : ∀ {x : LocalVariable} {u : UnrestrictedValue}
-    {M : Memory} {S : LocalStack},
-    maps_var_to M x u →
-    step_local M (val u :: S) (StLoc x) (mem_update_local M x u) S
-  | step_stloc_ref : ∀ {x : LocalVariable} {r : Reference}
-    {M : Memory} {S : LocalStack},
-    maps_var_to M x r →
-    step_local M (ref_val r :: S) (StLoc x) (mem_update_local M x r) S
-  | step_borrow_loc : ∀ {x : LocalVariable} {v : Value}
-    {M : Memory} {S : LocalStack},
-    maps_var_to M x v →
-    step_local M S (BorrowLoc x) M (ref_val {|
-      root := x;
-      access_path := [ ];
-      mutability := mut
-    |} :: S)
-  | step_borrow_field : ∀ {x : LocalVariable} {f : FieldName} {r : Reference}
-    {M : Memory} {S : LocalStack},
-    step_local M (ref_val r :: S) (BorrowField f) M (ref_val (extend_ref r f) :: S)
-  | step_freeze_ref : ∀ {r : Reference}
-    {M : Memory} {S : LocalStack},
-    step_local M (ref_val r :: S) FreezeRef M ((ref_val (freeze_ref r)) :: S)
-  | step_read_ref : ∀ {r : Reference} {u : UnrestrictedValue}
-    {M : Memory} {S : LocalStack},
-    maps_ref_to M r u →
-    step_local M (ref_val r :: S) ReadRef M (val u :: S)
-  | step_write_ref : ∀ {r : Reference} {u : UnrestrictedValue}
-    {M : Memory} {S : LocalStack},
-    maps_ref_to M r u →
-    step_local M (val u :: ref_val r :: S) WriteRef (mem_update_ref M r u) S
-  | step_pop_u : ∀ {u : UnrestrictedValue}
-    {M : Memory} {S : LocalStack},
-    step_local M (val u :: S) Pop M S
-  | step_pop_ref : ∀ {r : Reference}
-    {M : Memory} {S : LocalStack},
-    step_local M (ref_val r :: S) Pop M S
-  | step_pack_r : ∀ {τ : StructType} {n : nat} {lov : list Value} {t : Tag}
-    {M : Memory} {S : LocalStack},
-    maps_struct_kind M τ resourceKind →
-    maps_struct_arity M τ n →
-    length lov = n →
-    fresh_tag M S t →
-    step_local M ((map val lov) ++ S) (Pack τ) M (val (resource t τ lov) :: S)
-  | step_pack_u : ∀ {τ : StructType} {n : nat} {lou : list UnrestrictedValue}
-    {M : Memory} {S : LocalStack},
-    maps_struct_kind M τ unrestrictedKind →
-    maps_struct_arity M τ n →
-    length lou = n →
-    step_local M ((map (fun x => (val (unrestrictiveValue x)))) lou) (Pack τ) M ((val (struct τ (map unrestrictiveValue lou))) :: S)
-  | step_unpack : ∀ {τ : StructType} {lov : list Value}
-    {M : Memory} {S : LocalStack},
-    step_local M (val (struct τ lov) :: S) Unpack M (map val lov ++ S)
-  | step_load_true : ∀ {M : Memory} {S : LocalStack},
-    step_local M S LoadTrue M (val true :: S)
-  | step_load_false : ∀ {M : Memory} {S : LocalStack},
-    step_local M S LoadFalse M (val false :: S)
-  | step_load_u64 : ∀ {M : Memory} {S : LocalStack} {n : UnsignedInt64},
-    step_local M S (LoadU64 n) M (val n :: S)
-  | step_load_address : ∀ {M : Memory} {S : LocalStack} {a : AccountAddress},
-    step_local M S (LoadAddress a) M (val a :: S)
-  | step_load_bytes : ∀ {M : Memory} {S : LocalStack} {b : Bytes},
-    step_local M S (LoadBytes b) M (val b :: S)
-  | step_op : ∀ {op : OpCode} {n : nat} {lou : list UnrestrictedValue}
-    {M : Memory} {S : LocalStack},
-    op_arity op n →
-    length lou = n →
-    step_local M (map (fun x => (val (unrestrictiveValue x))) lou ++ S) op M (val (opcode_to_op op lou) :: S)
-  .
-
-(** Execution sequence  *)
-Record state := {
-  mem : Memory;
-  stack : LocalStack;
-}.
+Require Import Resources.small_step.
 
 Record StackRef := {
   stack_root : nat;
@@ -201,23 +115,18 @@ stack_maps_to s.(stack) r v -> state_maps_to s (inr r) v.
 Axiom state_maps_to_stack_compat1 : ∀ (s : state) (r : StackRef) (v : Value),
 state_maps_to s (inr r) v -> stack_maps_to s.(stack) r v.
 
-Definition tag_consistent (s : state) : Prop :=
+Definition tag_consistent' (s : state) : Prop :=
   ∀ (l1 l2 : state_loc) (c1 c2 : Resource),
     state_maps_to s l1 c1 →
     state_maps_to s l2 c2 →
     tag_of c1 = tag_of c2 →
     l1 = l2.
 
-Inductive step : state → state → Prop :=
-  | step_c : ∀ {s0 s1 : state} {i : Instr},
-    step_local s0.(mem) s0.(stack) i s1.(mem) s1.(stack) →
-    step s0 s1.
-
-Theorem step_preserve_tag_consistent :
+Theorem step_preserve_tag_consistent' :
 ∀ (s0 s1 : state),
-  tag_consistent s0 →
+  tag_consistent' s0 →
   step s0 s1 →
-  tag_consistent s1.
+  tag_consistent' s1.
 Proof.
   intros s0 s1 Hc Hs.
   destruct s0. destruct s1.
@@ -225,7 +134,7 @@ Proof.
   inversion H.
   + admit.
   (* cploc *)
-  + unfold tag_consistent. intros.
+  + unfold tag_consistent'. intros.
     destruct l1; destruct l2.
       ++ assert (state_maps_to s0 (inl r) c1). {
         apply state_maps_to_mem_compat1 in H6.
@@ -238,9 +147,9 @@ Proof.
         rewrite H0.
         assumption.
       }
-      unfold tag_consistent in Hc.
+      unfold tag_consistent' in Hc.
       apply Hc with (l1:=inl r) (l2:=inl r0) (c1:=c1) (c2:=c2); assumption.
-      ++ unfold tag_consistent in Hc.
+      ++ unfold tag_consistent' in Hc.
         apply state_maps_to_mem_compat1 in H6.
         rewrite <- H0 in H6.
         apply state_maps_to_mem_compat0 in H6.
@@ -264,7 +173,7 @@ Proof.
           apply Hc in H6; auto.
           inversion H6.
         }
-      ++ unfold tag_consistent in Hc.
+      ++ unfold tag_consistent' in Hc.
         apply state_maps_to_mem_compat1 in H7.
         rewrite <- H0 in H7.
         apply state_maps_to_mem_compat0 in H7.
@@ -288,7 +197,7 @@ Proof.
           apply Hc in H7; auto.
           inversion H7.
         }
-      ++ unfold tag_consistent in Hc.
+      ++ unfold tag_consistent' in Hc.
         apply state_maps_to_stack_compat1 in H6.
         apply state_maps_to_stack_compat1 in H7.
         rewrite <- H4 in H6, H7.
